src/CSL/RefinementAdequacy.v
@@ -1,0 +1,95 @@
+Require Import Spec.Proc.
+Require Import Spec.ProcTheorems.
+Require Import Spec.Abstraction.
+Require Import Spec.Layer.
+Require Import Helpers.RelationAlgebra.
+Require Import Helpers.RelationTheorems.
+Require Import Helpers.RelationRewriting.
+Require Import CSL.WeakestPre CSL.Refinement CSL.Adequacy.
+From iris.algebra Require Import auth frac agree gmap list.
+From iris.base_logic.lib Require Import invariants.
+From iris.proofmode Require Import tactics.
+Unset Implicit Arguments.
+
+Import RelationNotations.
+Definition pool_map_incl {OpT} (tp1: gmap nat (@procT OpT)) (tp2: thread_pool OpT) :=
+  ∀ j e, tp1 !! j = Some e → tp2 !! j = Some e.
+
+Theorem wp_recovery_refinement {T R} OpTa OpTc Σ (Λa: Layer OpTa) (Λc: Layer OpTc) `{invPreG Σ} s
+        (ea: proc OpTa T) (ec: proc OpTc T) (rec: proc OpTc R)
+        φ (absr: Λa.(State) → Λc.(State) → unit → Prop) E :
+  nclose sourceN ⊆ E →
+  (∀ (σ1a: Λa.(State)) σ1c,
+      absr σ1a σ1c tt →
+      (∀ `{Hinv : invG Σ} `{Hcfg: cfgG OpTa Λa Σ},
+          (|={⊤}=> ∃ stateI : State Λc → iProp Σ,
+             let _ : irisG OpTc Λc Σ := IrisG _ _ _ Hinv stateI in
+             stateI σ1c ∗ source_ctx ([existT _ ea], σ1a)
+               ∗ WP ec @ s; ⊤ {{ v, O ⤇ of_val v
+                    ∗ (∀ σ2c, stateI σ2c ={⊤,E}=∗ ∃ σ2a, source_state σ2a ∗ ⌜absr σ2a σ2c tt⌝)}}
+                              ∗ (∀ σ2c, stateI σ2c ={⊤,E}=∗ ∃ tp σ2a, source_pool_map tp
+                                         ∗ source_state σ2a ∗ ⌜φ tp σ2a σ2c⌝))%I)) →
+  (∀ `{Hinv : invG Σ} `{Hcfg: cfgG OpTa Λa Σ}
+     tp1 tp1' σ1a σ1c σ1c'
+     (Hφ: φ tp1 σ1a σ1c)
+     (Htp_sub: pool_map_incl tp1 tp1')
+     (Hcrash: Λc.(crash_step) σ1c σ1c' tt),
+     (|={⊤}=> ∃ stateI : State Λc → iProp Σ,
+       let _ : irisG OpTc Λc Σ := IrisG _ _ _ Hinv stateI in
+       stateI σ1c' ∗ source_ctx (tp1', σ1a)
+              ∗ WP rec @ s; ⊤ {{ v, (∀ σ2c, stateI σ2c ={⊤,E}=∗
+                   ∃ σ2a σ2a', source_state σ2a ∗ ⌜Λa.(crash_step) σ2a σ2a' tt ∧ absr σ2a' σ2c tt⌝)}}
+                              ∗ (∀ σ2c, stateI σ2c ={⊤,E}=∗ ∃ tp σ2a, source_pool_map tp
+                                         ∗ source_state σ2a ∗ ⌜φ tp σ2a σ2c⌝))%I) →
+  crash_refines absr Λc ec (rec_singleton rec) (Λa.(exec) ea)
+                (and_then (Λa.(exec_halt) ea) (fun _ => Λa.(crash_step))).
+Proof.
+  intros Hsub Hwp_e Hwp_rec.
+  assert (∀ σ1a σ1c, absr σ1a σ1c tt → recv_adequate s ec rec σ1c
+                          (λ v' σ2c', ∃ σ2a, exec Λa ea σ1a σ2a (existT _ v') ∧
+                                             absr σ2a σ2c' tt)
+                          (fun _ => True)).
+  { intros.
+    eapply wp_recovery_adequacy with
+        (φinv := fun σ2c => ∃ tp2 tp2' σ2a efs, pool_map_incl tp2 tp2' ∧ φ tp2 σ2a σ2c
+                                                ∧ exec_partial Λa ea σ1a σ2a tp2'); eauto.
+    - iIntros (Hinv).
+      assert (Inhabited Λa.(State)).
+      { eexists; eauto. }
+      iMod Hwp_e as (stateI) "[Hstate [#Hsrc [H Hφ]]]"; eauto.
+      iExists stateI. iIntros "{$Hstate} !>".
+      iSplitL "H".
+      * iApply wp_wand_l; iFrame "H". iIntros (v') "[Hmapsto Hopen]".
+        iIntros (σ2c') "Hstate".
+        iMod ("Hopen" with "Hstate") as (σ2a) "(Hstate&%)".
+        iInv "Hsrc" as (tp' σ') ">[Hauth Hp]" "_".
+        iDestruct "Hp" as %Hp. rewrite //= in Hp.
+        iDestruct (source_state_reconcile with "Hstate Hauth") as %Hstate; subst.
+        iDestruct (source_thread_reconcile with "Hmapsto Hauth") as %Hlookup; subst.
+        apply take_drop_middle in Hlookup.
+
+        iApply fupd_mask_weaken; first by set_solver+.
+        iPureIntro. exists σ'; split; eauto.
+        rewrite -Hlookup //= /of_val in Hp.
+        eapply exec_partial_finish; eauto.
+      * iIntros (σ2c') "Hstate".
+        iMod ("Hφ" with "Hstate") as (tp2 σ2a) "(Hpool&Hstate&%)".
+        iInv "Hsrc" as (tp' σ') ">[Hauth Hp]" "_".
+        iDestruct "Hp" as %Hp. rewrite //= in Hp.
+        iDestruct (source_state_reconcile with "Hstate Hauth") as %Hstate; subst.
+        iDestruct (source_pool_map_reconcile with "Hpool Hauth") as %Hpool; subst.
+
+        iApply fupd_mask_weaken; first by set_solver+.
+        iPureIntro. exists tp2, tp', σ'; split; eauto.
+    - admit.
+  }
+  split.
+  - rewrite /refines.
+    intros σ1a σ2c (T'&v) ([]&σ1c&Habsr&Hexec).
+    edestruct H0; eauto.
+    edestruct (recv_adequate_normal_result) as (v'&Heq_val&σ2a&HexecA&Habsr'); eauto.
+    do 3 eexists; eauto.
+    do 3 eexists; eauto.
+    econstructor; eauto.
+  -
+Abort.
